Aesop/Search/Queue/Class.lean
@@ -1,0 +1,24 @@
+/-
+Copyright (c) 2022 Jannis Limperg. All rights reserved.
+Released under Apache 2.0 license as described in the file LICENSE.
+Authors: Jannis Limperg
+-/
+
+import Aesop.Tree
+
+open Lean
+
+namespace Aesop
+
+class Queue (Q : Type) where
+  init : BaseIO Q
+  addGoals : Q → Array GoalRef → BaseIO Q
+  popGoal : Q → BaseIO (Option GoalRef × Q)
+  format : Q → MetaM MessageData
+
+namespace Queue
+
+def init' [Queue Q] (grefs : Array GoalRef) : BaseIO Q := do
+  addGoals (← init) grefs
+
+end Aesop.Queue
