Aesop/Search/SearchM.lean
@@ -6,7 +6,7 @@ Authors: Jannis Limperg
 
 import Aesop.Options
 import Aesop.Search.Expansion.Simp.Basic
-import Aesop.Search.Queue
+import Aesop.Search.Queue.Class
 import Aesop.Profiling
 import Aesop.RuleSet
 
