tests/run/Strategy.lean
@@ -1,0 +1,34 @@
+/-
+Copyright (c) 2022 Jannis Limperg. All rights reserved.
+Released under Apache 2.0 license as described in the file LICENSE.
+Authors: Jannis Limperg
+-/
+
+import Aesop
+
+set_option aesop.check.all true
+
+@[aesop 50% constructors]
+inductive I₁
+  | ofI₁ : I₁ → I₁
+  | ofTrue : True → I₁
+
+example : I₁ := by
+  aesop
+
+example : I₁ := by
+  aesop (options := { strategy := .bestFirst })
+
+example : I₁ := by
+  aesop (options := { strategy := .breadthFirst })
+
+example : I₁ := by
+  fail_if_success
+    aesop (options :=
+      { strategy := .depthFirst,
+        maxRuleApplicationDepth := 0,
+        maxRuleApplications := 10,
+        terminal := true })
+  aesop (options :=
+    { strategy := .depthFirst,
+      maxRuleApplicationDepth := 10 })
